Remove [EF_builtin] and the associated [ef_inline]

arm/PrintAsm.ml
@@ -623,8 +623,6 @@ let print_instruction oc = function
       2 + List.length tbl
   | Pbuiltin(ef, args, res) ->
       begin match ef with
-      | EF_builtin(name, sg) ->
-          print_builtin_inline oc (extern_atom name) args res
       | EF_vload chunk ->
           print_builtin_vload oc chunk args res
       | EF_vstore chunk ->
