cfrontend/C2C.ml
@@ -739,9 +739,7 @@ let convertFundecl env (sto, id, ty, optinit) =
   let ef =
     if id.name = "malloc" then EF_malloc else
     if id.name = "free" then EF_free else
-    if List.mem_assoc id.name builtins.functions
-    then EF_builtin(id', sg)
-    else EF_external(id', sg) in
+    EF_external(id', sg) in
   (id', Gfun(External(ef, args, res)))
 
 (** Initializers *)
