backend/Selection.v
@@ -128,8 +128,7 @@ Fixpoint sel_exprlist (al: list Cminor.expr) : exprlist :=
 
 Inductive call_kind `{sc_ops: SyntaxConfigOps} : Type :=
   | Call_default
-  | Call_imm (id: ident)
-  | Call_builtin (ef: external_function).
+  | Call_imm (id: ident).
 
 Definition expr_is_addrof_ident (e: Cminor.expr) : option ident :=
   match e with
@@ -144,15 +143,7 @@ Context `{Hsc: SyntaxConfiguration}.
 Definition classify_call (ge: Cminor.genv) (e: Cminor.expr) : call_kind :=
   match expr_is_addrof_ident e with
   | None => Call_default
-  | Some id =>
-      match Genv.find_symbol ge id with
-      | None => Call_imm id
-      | Some b =>
-          match Genv.find_funct_ptr ge b with
-          | Some(External ef) => if ef_inline ef then Call_builtin ef else Call_imm id
-          | _ => Call_imm id
-          end
-      end
+  | Some id => Call_imm id
   end.
 
 (** Conversion from Cminor statements to Cminorsel statements. *)
@@ -166,7 +157,6 @@ Fixpoint sel_stmt (ge: Cminor.genv) (s: Cminor.stmt) : stmt :=
       match classify_call ge fn with
       | Call_default => Scall optid sg (inl _ (sel_expr fn)) (sel_exprlist args)
       | Call_imm id  => Scall optid sg (inr _ id) (sel_exprlist args)
-      | Call_builtin ef => Sbuiltin optid ef (sel_exprlist args)
       end
   | Cminor.Sbuiltin optid ef args =>
       Sbuiltin optid ef (sel_exprlist args)
